\documentclass{article}
\usepackage[utf8]{inputenc}
\usepackage[margin=0.5in]{geometry}
\usepackage{amsmath}

\title{61DM HW 1 Problem 1}
\author{Edwin Trejo}

\begin{document}

\maketitle

\section{Problem}
 Use the principle of mathematical induction to check that 
    \[\sum_{j=1}^{n}j^3=\frac{n^{2}(n+1)^2}{4}, n\in \mbox{\textbf{Z}}^+\]

\section{Solution}
First, we ensure the proposition is true for \(n=1\):
\[\sum_{j=1}^{1}j^3=1^3=1\]
\[\frac{1^{2}(1+1)^2}{4}=\frac{4}{4}=1\]
\[1=1\]
So, the proposition holds for \(n=1\). Next, we assume the proposition is true for all \(n=k\):
\[\sum_{j=1}^{k}j^3=\frac{k^{2}(k+1)^2}{4}, k\in \mbox{\textbf{Z}}^+\]
Now, we show the proposition is true for all \(n=k+1\), that is:
\[\sum_{j=1}^{k+1}j^3=\frac{(k+1)^{2}(k+2)^2}{4}, k\in \mbox{\textbf{Z}}^+\]
Beginning with the left-hand side:
\begin{align*}
    \sum_{j=1}^{k+1}j^3 &= \sum_{j=1}^{k}j^3 + (k+1)^3 \\
    &= \frac{k^{2}(k+1)^2}{4} + (k+1)^3 \ \ \ \ [\mbox{by assumption}] \\
    &= \frac{k^{2}(k+1)^2}{4} + \frac{4(k+1)(k+1)^2}{4} \\
    &= \frac{k^{2}(k+1)^2 + 4(k+1)(k+1)^2}{4} \\ 
    &= \frac{(k+1)^2(k^2+4k+4)}{4} \\
    &= \frac{(k+1)^2(k+2)^2}{4} \\
\end{align*}
Which is equal to the right-hand side. Therefore, since the proposition holds for \(n=1\) and all \(n=k+1\), it is true for all \(n\in\mbox{\textbf{Z}}^+\)

\end{document}